Prove last composition lemmas. Add Let w/ CPS

src/named/Let.v
@@ -1,245 +1,73 @@
-Require Import mathcomp.ssreflect.all_ssreflect.
 Set Implicit Arguments.
-Unset Strict Implicit.
-Unset Printing Implicit Defensive.
 Set Bullet Behavior "Strict Subproofs".
 
-
-From Ltac2 Require Import Ltac2.
-Set Default Proof Mode "Classic".
+Require Import String List.
+Import ListNotations.
+Open Scope string.
+Open Scope list.
 From Utils Require Import Utils.
-From Named Require Import Exp Core.
-From Named Require Import IExp IRule ICore ICompilers Subst STLC Tactics.
-Import Exp.Notations.
-Import IExp.Notations IRule.Notations ARule.Notations.
-Require Import String.
-
+From Named Require Import Core Compilers Elab ElabCompilers
+     ElabCompilersWithPrefix SimpleVSubst SimpleVCPS Matches.
+Module Pre := ElabWithPrefix.
+Import Core.Notations.
+Import CompilerDefs.Notations.
 
 Require Coq.derive.Derive.
 
-Set Default Proof Mode "Ltac2".
-
- Lemma elab_args_cons_ex' l c : forall s args (es:list Exp.exp) c' name e ee t,
-    fresh name c' ->
-    (* these arguments are last so that proof search unifies existentials
-       from the other arguments first*)
-    elab_args l c s args es c' ->
-    (* TODO: some langs want this first, some want it later.
-       Which is better?*)
-    elab_term l c e ee (Exp.apply_subst (with_names_from c' es) t) ->
-    Core.wf_sort (strip_args l) c' t ->
-    elab_args l c (e::s) (name::args) (ee::es) ((name,t)::c').
- Proof.
-   eauto with judgment.
- Qed.
-(* TODO: let/k? *)
- Definition stlc_let :=
-  [::
-  [:> "G" : #"env",
-      "A" : #"ty" %"G",
-      "B" : #"ty" %"G",
-      "e" : #"el" %"G" %"A",
-      "body" : #"el" (#"ext" %"G" %"A") (#"ty_subst" #"wkn" %"B")
-      ----------------------------------------------- ("let beta")
-      #"let" %"e" %"body" = #"app" (#"lambda" %"body")  %"e"
-      : #"el" %"G" %"B"
-     ];
+Definition let_lang_def : lang :=
+  {[l
   [:| "G" : #"env",
-      "A" : #"ty" %"G",
-      "B" : #"ty" %"G",
-      "e" : #"el" %"G" %"A",
-      "body" : #"el" (#"ext" %"G" %"A") (#"ty_subst" #"wkn" %"B")
+      "A" : #"ty",
+      "B" : #"ty",
+      "e" : #"exp" "G" "A",
+      "e'" : #"exp" (#"ext" "G" "A") "B"
       -----------------------------------------------
-      #"let" "e" "body"  : #"el" %"G" %"B"
-  ]]%irule++stlc.
-  
-Derive elab_stlc_let
-       SuchThat (elab_lang stlc_let elab_stlc_let)
-       As elab_stlc_let_pf.
-Proof.
-  repeat (elab easy_le_tac);
-  repeat (elab easy_le_tac).
-  (*TODO: figure out why 2 repeats *)
-Qed.
-  
+      #"let" "e" "e'" : #"exp" "G" "B"
+  ];
+  [:= "G" : #"env",
+      "A" : #"ty",
+      "B" : #"ty",
+      "v" : #"val" "G" "A",
+      "e" : #"exp" (#"ext" "G" "A") "B"
+      ----------------------------------------------- ("eval let")
+      #"let" (#"ret" "v") "e"
+      = #"exp_subst" (#"snoc" #"id" "v") "e"
+      : #"exp" "G" "B"
+  ];
+  [:= "G" : #"env", 
+      "A" : #"ty",
+      "B" : #"ty",
+      "e" : #"exp" "G" "A",
+      "e'" : #"exp" (#"ext" "G" "A") "B",
+      "G'" : #"env",
+      "g" : #"sub" "G'" "G"
+      ----------------------------------------------- ("let_subst")
+      #"exp_subst" "g" (#"let" "e" "e'")
+      = #"let" (#"exp_subst" "g" "e")
+         (#"exp_subst" (#"snoc" (#"cmp" #"wkn" "g") #"hd") "e'")
+      : #"exp" "G'" "B"
+  ]
+  ]}.
 
-Instance elab_stlc_let_inst : Elaborated stlc_let :=
-  {
-  elaboration := elab_stlc_let;
-  elab_pf := elab_stlc_let_pf;
-  }.
+Derive let_lang
+       SuchThat (Pre.elab_lang (exp_subst++value_subst) let_lang_def let_lang)
+       As let_lang_wf.
+Proof. auto_elab. Qed.
+#[export] Hint Resolve let_lang_wf : elab_pfs.
 
-(*
-(* TODO: general-purpose lemma that macro-like languages
-   like this can be compiled away
- *)
-Definition compile_macro_sort (c:string) args : sort := scon c (map var args).
-
-(*TODO:move helper somewhere; duped from CPS*)
-Definition lookup_args l n :=
-  get_rule_args ( named_list_lookup (ARule.sort_rule [::] [::]) l n).
-Definition compile_macro
-           (* macro components *)
-           name e
-           (c : string) (args : list string) : exp :=
-    if c == name
-    then e
-    else con c (map var (lookup_args elab_stlc c)).
-  
-Derive elab_compile_macro
-  SuchThat
-  (forall target c name t args e eq_name (elab_macro elab_target : ARule.lang),
-    let macro_ext :=
-        [:: (eq_name,term_le c (con name (map var args)) e t);
-        (name,term_rule c args t)]
-    in
-    let compiler := ICompilers.make_compiler compile_macro_sort
-                                  (compile_macro name e)
-                                  (strip_args (elab_macro++elab_target))
-    in
-    elab_lang target elab_target ->
-    elab_lang (macro_ext ++ target) (elab_macro++elab_target) ->
-    elab_preserving_compiler elab_target
-                             compiler
-                             (elab_compile_macro ...)
-                             (elab_macro++elab_target))
-    As compile_macro_preserving.
- *)
-
-(*TODO: copied from CPS; should have definitive version *)
-Require Import Recognizers.
-
-Ltac2 has_evar (c : constr) :=
-  Control.plus (fun ()=> ltac1:(c|-has_evar c) (Ltac1.of_constr c); true)
-               (fun _=> false).
-
-Ltac2 reflexivity_no_evars () :=
-  match! goal with
-    [|- _ ?a ?b] =>
-    match Bool.or (has_evar a) (has_evar b) with
-    | true => Control.backtrack_tactic_failure "found evars in goal terms"
-    | false => reflexivity
-    end
+Definition let_cps_def : compiler :=
+  match # from (let_lang) with
+  | {{e #"let" "G" "A" "B" "e" "e'"}} =>
+    bind_k 1 "e" "A"
+    {{e#"blk_subst" (#"snoc" (#"snoc" {wkn_n 2} #"hd") {ovar 1}) "e'"}}
   end.
 
-(*TODO: I think I should make sure this never errors, might
-  be what's causing double-repeat issues*)
-Import Control.
-Ltac2 rec elab () :=
-  simpl;
-  match! goal with
-  | [|- elab_lang nil _] => constructor; enter elab
-  | [|- elab_lang _ _] => (Control.plus (fun () => apply elab_pf) (fun _ => constructor)); enter elab
-  | [tll : ARule.lang|- elab_rule ?l _ _] =>
-    let tll := Control.hyp tll in
-    (*TODO: precompute this? definitely at least needs simpl but maybe not here
-    let n := Std.eval_vm None constr:(size $tll - size $l) in*)
-    ltac1:(l tll|-change l with (nth_tail (size tll - size l) tll))
-            (Ltac1.of_constr l) (Ltac1.of_constr tll);
-    constructor; enter elab
-  | [|- elab_ctx _ _ _] => constructor;enter elab
-  | [|- elab_args _ _ _ _ _ [::]] => apply elab_args_nil;enter elab
-  | [|- elab_args _ _ _ (?n::_) _ ((?n,?t)::_)] =>
-      apply elab_args_cons_ex;enter elab
-  | [|- elab_args _ _ _ _ _ ((?n,?t)::_)] =>
-      eapply elab_args_cons_im;enter elab
-  (* special case to force existentials to the empty list*)
-  | [|- elab_subst _ _ _ (with_names_from [::] ?l) [::]] =>
-        assert ($l = [::]) > [reflexivity | apply elab_subst_nil;enter elab]
-  | [|- elab_subst _ _ _ _ [::]] => apply elab_subst_nil;enter elab
-  | [|- elab_subst _ _ ((?n,?e)::_) ((?n,?ee)::_) ((?n,?t)::_)] =>
-      apply elab_subst_cons_ex > [solve_fresh ()| | |]; enter elab
-  | [|- elab_subst _ _ _ ((?n,?ee)::_) ((?n,?t)::_)] =>
-      eapply elab_subst_cons_im > [solve_fresh ()| | |]; enter elab
-  | [|- elab_sort _ _ _ _] => apply elab_sort_by'; enter elab
-  | [|- Core.le_args _ _ _ _ _] =>constructor; enter elab
-  (* TODO: tmp; try shelving any wfness side-conditions; do elab first*)
-  | [|- Core.wf_args _ _ _ _] =>(*first [apply wf_args_no_conv_recognizes; vm_compute; reflexivity
-                                      | apply Core.wf_args_cons
-                                      | apply Core.wf_args_nil]*)()
-  | [|- Core.wf_subst _ _ _ _] =>(*constructor*) ()
-  | [|- Core.wf_sort ?l ?c ?t] =>
-    (*time: mean ~0.03 high ~0.3*)
-    match Bool.or (has_evar l) (Bool.or (has_evar c) (has_evar t)) with
-    | true => ()
-    | false => apply wf_sort_no_conv_recognizes; vm_compute; reflexivity
-    end
-  | [|- Core.wf_term _ _ (Exp.var _) _] =>
-    eapply Core.wf_term_conv > [apply Core.wf_term_var; solve_in() |enter elab ..]
-  | [|- Core.wf_term ?l ?c ?e ?t] =>
-    match has_evar '(Core.wf_term $l $c $e $t) with
-    | true => ()
-    | false => apply wf_term_no_conv_recognizes; vm_compute; reflexivity
-    end
-    (*eapply Core.wf_term_conv> [ | eapply Core.wf_term_by' | ]*)
-  | [|- elab_term _ _ (var _) _ _] =>
-    eapply elab_term_conv > [apply elab_term_var; solve_in() |enter elab ..]
-  | [|- elab_term _ _ _ (Exp.var _) _] =>
-                 (*
-TODO: no speedup vs this;
-maybe could assrt wf ctx to avoid wf sort assumptions?
-eapply elab_term_conv > [apply elab_term_var; solve_in() | enter elab ..]*)
-                  apply elab_term_conv_var ; enter elab 
-  | [|- elab_term _ _ (con _ _) _ _] => 
-    eapply elab_term_conv > [apply elab_term_by';enter elab | enter elab ..]
-  | [|- elab_term _ _ _ (Exp.con _ _) _] => 
-    eapply elab_term_conv > [apply elab_term_by';enter elab | enter elab ..]
-  | [|- elab_term _ _ ?e ?ee _] =>
-    match Bool.and (is_evar e) (is_evar ee) with
-    | true => ()
-    | false => ()
-    end
-  | [|- is_true((?n,?e)\in ?l)]=> 
-      assert ($e = named_list_lookup $e $l $n); cbv; solve[auto]
-  | [|- is_true (_ \in _)] => solve_in ()
-  | [|- is_true (fresh _ _)] => solve_fresh ()
-  | [|- is_true (_ \notin _)] => solve_fresh ()
-  | [|- is_true (subseq _ _)] => vm_compute; reflexivity
-  | [|- is_true true] => reflexivity
-  | [|- len_eq _ _] => constructor;enter elab
-  | [|- _ = _] => try (solve[reflexivity| cbv; f_equal])
-  | [|- Core.le_term _ _ _ _ _]=>
-    (*time: mean ~0.02 high ~0.3*)
-    try (solve[apply Core.le_term_by_nameless; vm_compute; reflexivity
-              | reflexivity_no_evars ()])
-  | [|- Core.le_sort _ _ _ _]=>
-    (*time: mean ~0.3 high ~0.5*)
-    try (solve[apply Core.le_sort_by_nameless; vm_compute; reflexivity
-              | reflexivity_no_evars()])
-  | [ |-  elab_preserving_compiler _ ((_,sort_case _ _)::_) _ _]=>
-    apply preserving_compiler_sort';enter elab
-  | [ |-  elab_preserving_compiler _ ((_,term_case _ _)::_) _ _]=>
-    apply preserving_compiler_term';enter elab
-  | [ |-  elab_preserving_compiler _ _ _ _]=>
-    constructor;enter elab
-end.
-
-
-Definition compile_let_sort (c:string) args : sort := scon c (map var args).
-Arguments compile_let_sort c args/.
-
-(*TODO:move helper somewhere; duped from CPS*)
-Definition lookup_args l n :=
-  get_rule_args ( named_list_lookup (ARule.sort_rule [::] [::]) l n).
-
-
-Definition compile_let (c : string) (args : list string) : exp :=
-  if c == "let"%string
-  then con "app" [:: var "e"; con "lambda" [:: var "body"]]
-  else con c (map var (lookup_args elab_stlc c)).
-Arguments compile_let c args /.
-
-
-Derive elab_compile_let
-       SuchThat (elab_preserving_compiler
-                   elab_stlc
-                   (make_compiler compile_let_sort
-                                  compile_let
-                                  (strip_args elab_stlc_let))
-                   elab_compile_let
-                   elab_stlc_let)
-       As elab_compile_let_preserving.
-Proof.
-  (* TODO: use Tactics.elab easy_le_tac.*)
-  repeat (elab()).
-Qed.
+Derive let_cps
+       SuchThat (elab_preserving_compiler cps_subst
+                                          (cps_lang ++ block_subst ++ value_subst)
+                                          let_cps_def
+                                          let_cps
+                                          let_lang)
+       As let_cps_preserving.
+Proof. auto_elab_compiler. Qed.
+#[export] Hint Resolve let_cps_preserving : elab_pfs.
