src/named/CompilerTools.v
@@ -1,0 +1,345 @@
+Set Implicit Arguments.
+Set Bullet Behavior "Strict Subproofs".
+
+Require Import String List.
+Import ListNotations.
+Open Scope string.
+Open Scope list.
+From Utils Require Import Utils.
+From Named Require Import Core Compilers Elab ElabCompilers ElabCompilersWithPrefix.
+Import Core.Notations.
+(*TODO: repackage this in compilers*)
+Import CompilerDefs.Notations.
+
+Require Coq.derive.Derive.
+
+Lemma elab_preserving_compiler_embed cmp_pre tgt cmp ecmp src tgt'
+    : elab_preserving_compiler cmp_pre tgt cmp ecmp src ->
+      incl tgt tgt' ->
+      elab_preserving_compiler cmp_pre tgt' cmp ecmp src.
+Proof.
+  induction 1; basic_goal_prep; constructor; basic_core_crush.
+  eapply eq_sort_lang_monotonicity; eauto.
+  eapply eq_term_lang_monotonicity; eauto.
+Qed.
+Hint Resolve elab_preserving_compiler_embed : auto_elab.
+
+
+Lemma strengthen_named_list_lookup {A} (cmp : named_list A) n
+  : forall cmp', incl cmp cmp' ->
+                 all_fresh cmp' ->
+                 In n (map fst cmp) ->
+                 named_list_lookup_err cmp' n = named_list_lookup_err cmp n.
+Proof.
+  induction cmp; basic_goal_prep;  symmetry; basic_utils_crush.
+  my_case neq (n =? s); basic_goal_prep; basic_utils_crush.
+Qed.
+
+Lemma compile_strengthen_term_incl cmp e
+  : all_constructors (fun n => In n (map fst cmp)) e ->
+    forall cmp', incl cmp cmp' ->
+                 all_fresh cmp' ->
+                 compile cmp' e = compile cmp e.
+Proof.
+  induction e; basic_goal_prep; basic_core_crush.
+  erewrite strengthen_named_list_lookup; eauto.
+  case_match; basic_goal_prep;[| basic_core_crush].
+  case_match; basic_goal_prep;[| basic_core_crush].
+  f_equal.
+  f_equal.
+ 
+  revert dependent l.
+  induction l; basic_goal_prep; f_equal; firstorder.
+Qed.
+
+Lemma compile_strengthen_args_incl cmp e
+  : all (all_constructors (fun n => In n (map fst cmp))) e ->
+    forall cmp', incl cmp cmp' ->
+                 all_fresh cmp' ->
+                 compile_args cmp' e = compile_args cmp e.
+Proof.
+  induction e; basic_goal_prep;
+    f_equal; firstorder eauto using compile_strengthen_term_incl.
+Qed.
+Hint Rewrite compile_strengthen_args_incl : lang_core.
+
+
+Lemma compile_strengthen_sort_incl cmp e
+  : all_constructors_sort (fun n => In n (map fst cmp)) e ->
+    forall cmp', incl cmp cmp' ->
+                 all_fresh cmp' ->
+                 compile_sort cmp' e = compile_sort cmp e.
+Proof.
+  induction e; basic_goal_prep; basic_core_crush.
+  erewrite strengthen_named_list_lookup; eauto.
+  case_match; basic_goal_prep;[| basic_core_crush].
+  case_match; basic_goal_prep;[basic_core_crush|].
+  f_equal.
+  f_equal.
+  apply compile_strengthen_args_incl; eauto.
+Qed.
+
+
+Lemma compile_strengthen_ctx_incl cmp e
+  : all_constructors_ctx (fun n => In n (map fst cmp)) e ->
+    forall cmp', incl cmp cmp' ->
+                 all_fresh cmp' ->
+                 compile_ctx cmp' e = compile_ctx cmp e.
+Proof.
+  induction e; basic_goal_prep;
+    f_equal; [f_equal|]; firstorder eauto using compile_strengthen_sort_incl.
+Qed.
+
+Fixpoint constructor_names (l:lang) : list string :=
+  match l with
+  | (n,term_rule _ _ _)::l' => n::(constructor_names l')
+  | (n,sort_rule _ _)::l' => n::(constructor_names l')
+  | _::l' => constructor_names l'
+  |[] => []
+  end.
+
+Lemma preserving_compiler_constructor_names tgt cmp src
+  : preserving_compiler tgt cmp src ->
+    map fst cmp = constructor_names src.
+Proof.
+  induction 1; basic_goal_prep; basic_core_crush.
+Qed.
+
+Lemma sort_rule_in_constructor_names n c args l
+  : In (n, sort_rule c args) l -> In n (constructor_names l).
+Proof.
+  induction l; basic_goal_prep; basic_core_crush.
+  case_match; basic_core_crush.
+Qed.
+Hint Resolve sort_rule_in_constructor_names : lang_core.
+
+
+Lemma term_rule_in_constructor_names n c args t l
+  : In (n, term_rule c args t) l -> In n (constructor_names l).
+Proof.
+  induction l; basic_goal_prep; basic_core_crush.
+  case_match; basic_core_crush.
+Qed.
+Hint Resolve term_rule_in_constructor_names : lang_core.
+
+Local Lemma all_constructors_from_wf src
+  : (forall c t,
+        wf_sort src c t ->
+        all_constructors_sort (fun n0 : string => In n0 (constructor_names src)) t)
+    /\ (forall c e t,
+           wf_term src c e t ->
+           all_constructors (fun n0 : string => In n0 (constructor_names src)) e)
+    /\ (forall c s c',
+           wf_args src c s c' ->
+           all (all_constructors (fun n0 : string => In n0 (constructor_names src))) s).
+Proof using.
+  intros; apply wf_judge_ind; basic_goal_prep;
+    with_rule_in_wf_crush.  
+Qed.
+
+Definition all_constructors_sort_from_wf src
+  := proj1 (all_constructors_from_wf src).
+#[export] Hint Resolve all_constructors_sort_from_wf : lang_core.
+
+Definition all_constructors_term_from_wf src 
+  := proj1 (proj2 (all_constructors_from_wf src)).
+#[export] Hint Resolve all_constructors_term_from_wf : lang_core.
+
+Definition all_constructors_args_from_wf src
+  := proj2 (proj2 (all_constructors_from_wf src)).
+#[export] Hint Resolve all_constructors_args_from_wf : lang_core.
+
+Lemma all_constructors_ctx_from_wf src c
+  : wf_ctx src c ->
+    all_constructors_ctx (fun n0 : string => In n0 (constructor_names src)) c.
+Proof.
+  induction 1; basic_goal_prep;
+    with_rule_in_wf_crush.
+Qed.
+#[export] Hint Resolve all_constructors_ctx_from_wf : lang_core.
+
+Require Import Compilers.
+
+
+
+Lemma strengthen_named_list_lookup' {A} (ecmp cmp : named_list A) n
+  : forall cmp', incl cmp cmp' ->
+                 all_fresh cmp' ->
+                 In n (map fst (ecmp++cmp)) ->
+                 named_list_lookup_err (ecmp++cmp') n = named_list_lookup_err (ecmp++cmp) n.
+Proof.
+  induction ecmp; basic_goal_prep; basic_utils_crush.
+  eapply strengthen_named_list_lookup; eauto.
+  my_case neq (n =? s); basic_goal_prep; basic_utils_crush.
+Qed.
+
+
+Lemma compile_strengthen_term_incl' ecmp cmp e
+  : all_constructors (fun n => In n (map fst (ecmp++cmp))) e ->
+    forall cmp', incl cmp cmp' ->
+                 all_fresh cmp' ->
+                 (compile (ecmp ++ cmp') e) = (compile (ecmp ++ cmp) e).
+Proof.
+  induction e; basic_goal_prep; basic_core_crush.
+  erewrite strengthen_named_list_lookup'; eauto.
+  case_match; basic_goal_prep;[| basic_core_crush].
+  case_match; basic_goal_prep;[| basic_core_crush].
+  f_equal.
+  f_equal.
+ 
+  revert dependent l.
+  induction l; basic_goal_prep; f_equal; firstorder.
+Qed.
+
+
+Lemma compile_strengthen_args_incl' ecmp cmp e
+  : all (all_constructors (fun n => In n (map fst (ecmp++cmp)))) e ->
+    forall cmp', incl cmp cmp' ->
+                 all_fresh cmp' ->
+                 (compile_args (ecmp ++ cmp') e) = (compile_args (ecmp ++ cmp) e).
+Proof.
+  induction e; basic_goal_prep;
+    f_equal; firstorder eauto using compile_strengthen_term_incl'.
+Qed.
+
+
+Lemma compile_strengthen_sort_incl' ecmp cmp e
+  : all_constructors_sort (fun n => In n (map fst (ecmp++cmp))) e ->
+    forall cmp', incl cmp cmp' ->
+                 all_fresh cmp' ->
+                 compile_sort (ecmp++cmp') e = compile_sort (ecmp++cmp) e.
+Proof.
+  induction e; basic_goal_prep; basic_core_crush.
+  erewrite strengthen_named_list_lookup'; eauto.
+  case_match; basic_goal_prep;[| basic_core_crush].
+  case_match; basic_goal_prep;[basic_core_crush|].
+  f_equal.
+  f_equal.
+  apply compile_strengthen_args_incl'; eauto.
+Qed.
+
+
+Lemma compile_strengthen_ctx_incl' ecmp cmp e
+  : all_constructors_ctx (fun n => In n (map fst (ecmp++cmp))) e ->
+    forall cmp', incl cmp cmp' ->
+                 all_fresh cmp' ->
+                 compile_ctx (ecmp++cmp') e = compile_ctx (ecmp++cmp) e.
+Proof.
+  induction e; basic_goal_prep;
+    f_equal; [f_equal|]; firstorder eauto using compile_strengthen_sort_incl'.
+Qed.
+
+Lemma constructor_names_app l l'
+  : constructor_names (l++l') = (constructor_names l) ++ (constructor_names l').
+Proof.
+  induction l; basic_goal_prep; try case_match; basic_goal_prep; basic_core_crush.
+Qed.
+
+
+Lemma elab_preserving_compiler_monotonicity cmp' cmp_pre tgt cmp ecmp src src_pre cmp_pre'
+  : ElabCompilers.elab_preserving_compiler tgt cmp' cmp_pre src_pre ->
+    elab_preserving_compiler cmp_pre tgt cmp ecmp src ->
+    wf_lang (src++src_pre) ->
+    incl cmp_pre cmp_pre' ->
+    all_fresh cmp_pre' ->
+    elab_preserving_compiler cmp_pre' tgt cmp ecmp src.
+Proof.
+  induction 2; basic_goal_prep; autorewrite with utils lang_core in *; constructor; intuition eauto.
+  {
+    erewrite compile_strengthen_ctx_incl'; eauto.
+    eapply all_constructors_ctx_weaken; cycle 1.
+    basic_core_crush.
+    simpl; intro.
+    erewrite !preserving_compiler_constructor_names; eauto.
+    eapply elab_compiler_implies_preserving.
+    eapply elab_compiler_prefix_implies_elab; eauto.
+  }
+  {
+    erewrite compile_strengthen_ctx_incl'; eauto.
+    erewrite compile_strengthen_sort_incl'; eauto.
+    {
+      eapply all_constructors_sort_weaken; cycle 1.
+      basic_core_crush.
+      simpl; intro.
+      erewrite !preserving_compiler_constructor_names; eauto.
+      eapply elab_compiler_implies_preserving.
+      eapply elab_compiler_prefix_implies_elab; eauto.
+    }
+    {
+      eapply all_constructors_ctx_weaken; cycle 1.
+      basic_core_crush.
+      simpl; intro.
+      erewrite !preserving_compiler_constructor_names; eauto.
+      eapply elab_compiler_implies_preserving.
+      eapply elab_compiler_prefix_implies_elab; eauto.
+    }
+  }
+  {
+    erewrite compile_strengthen_ctx_incl'; eauto.
+    erewrite compile_strengthen_sort_incl'; eauto.
+    erewrite (compile_strengthen_sort_incl' ecmp t2); eauto.
+    {
+      eapply all_constructors_sort_weaken; cycle 1.
+      basic_core_crush.
+      simpl; intro.
+      erewrite !preserving_compiler_constructor_names; eauto.
+      eapply elab_compiler_implies_preserving.
+      eapply elab_compiler_prefix_implies_elab; eauto.
+    }
+    {
+      eapply all_constructors_sort_weaken; cycle 1.
+      basic_core_crush.
+      simpl; intro.
+      erewrite !preserving_compiler_constructor_names; eauto.
+      eapply elab_compiler_implies_preserving.
+      eapply elab_compiler_prefix_implies_elab; eauto.
+    }
+    {
+      eapply all_constructors_ctx_weaken; cycle 1.
+      basic_core_crush.
+      simpl; intro.
+      erewrite !preserving_compiler_constructor_names; eauto.
+      eapply elab_compiler_implies_preserving.
+      eapply elab_compiler_prefix_implies_elab; eauto.
+    }
+  }
+  {
+    erewrite compile_strengthen_ctx_incl'; eauto.
+    erewrite compile_strengthen_sort_incl'; eauto.
+    erewrite (compile_strengthen_term_incl' ecmp e1); eauto.
+    erewrite (compile_strengthen_term_incl' ecmp e2); eauto.
+    {
+      eapply all_constructors_term_weaken; cycle 1.
+      basic_core_crush.
+      simpl; intro.
+      erewrite !preserving_compiler_constructor_names; eauto.
+      eapply elab_compiler_implies_preserving.
+      eapply elab_compiler_prefix_implies_elab; eauto.
+    }
+    {
+      eapply all_constructors_term_weaken; cycle 1.
+      basic_core_crush.
+      simpl; intro.
+      erewrite !preserving_compiler_constructor_names; eauto.
+      eapply elab_compiler_implies_preserving.
+      eapply elab_compiler_prefix_implies_elab; eauto.
+    }
+    {
+      eapply all_constructors_sort_weaken; cycle 1.
+      basic_core_crush.
+      simpl; intro.
+      erewrite !preserving_compiler_constructor_names; eauto.
+      eapply elab_compiler_implies_preserving.
+      eapply elab_compiler_prefix_implies_elab; eauto.
+    }
+    {
+      eapply all_constructors_ctx_weaken; cycle 1.
+      basic_core_crush.
+      simpl; intro.
+      erewrite !preserving_compiler_constructor_names; eauto.
+      eapply elab_compiler_implies_preserving.
+      eapply elab_compiler_prefix_implies_elab; eauto.
+    }
+  }
+Qed.
+Hint Resolve elab_preserving_compiler_monotonicity : auto_elab.
