src/named/ExampleProgram.v
@@ -1,0 +1,117 @@
+Set Implicit Arguments.
+Set Bullet Behavior "Strict Subproofs".
+
+Require Import String List.
+Import ListNotations.
+Open Scope string.
+Open Scope list.
+From Utils Require Import Utils.
+From Named Require Import Core Compilers Elab ElabCompilers ElabCompilersWithPrefix
+     SimpleVSubst SimpleVCPS SimpleEvalCtx SimpleEvalCtxCPS SimpleUnit NatHeap SimpleVCPSHeap
+     SimpleVFixCPS SimpleVCC SimpleVCCHeap SimpleVFix Matches CompilerTransitivity CompilerTools.
+Import Core.Notations.
+(*TODO: repackage this in compilers*)
+Import CompilerDefs.Notations.
+
+Require Coq.derive.Derive.
+
+Ltac solve_incl := 
+  solve [auto with utils
+        | apply use_compute_incl_lang; vm_compute; reflexivity].
+Ltac use_preserving_hint :=
+  eapply elab_preserving_compiler_embed;
+  [eapply elab_preserving_compiler_monotonicity;
+   [ eauto with elab_pfs| solve_incl|apply use_compute_all_fresh; vm_compute; reflexivity]
+  | solve_incl].
+
+(*TODO: put these hints with their subjects*)
+Hint Resolve cps_preserving : elab_pfs.
+Hint Resolve Ectx_cps_preserving : elab_pfs.
+Hint Resolve fix_cps_preserving : elab_pfs.
+
+Hint Resolve ElabCompilers.elab_preserving_compiler_nil : auto_elab.
+
+(*TODO: put in right place*)
+
+Import SumboolNotations.
+
+Definition case_eq_dec (r1 r2 : compiler_case) : {r1 = r2} + {~ r1 = r2}.
+  refine(match r1, r2 with
+         | sort_case args t, sort_case args' t' =>
+           SB! (list_eq_dec string_dec args args') SB&
+           (sort_eq_dec t t')
+         | term_case args t, term_case args' t' =>
+           SB! (list_eq_dec string_dec args args') SB&
+           (term_eq_dec t t')
+         | _,_ => _
+         end); autorewrite with utils lang_core; try intuition fail.
+  all: right.
+  all: intros; basic_core_crush.
+Defined.
+
+Definition compute_incl_compiler (l1 l2 : compiler) :=
+  if incl_dec (pair_eq_dec string_dec case_eq_dec) l1 l2 then true else false.
+
+Lemma use_compute_incl_compiler l1 l2
+  : compute_incl_compiler l1 l2 = true -> incl l1 l2.
+Proof.
+  unfold compute_incl_compiler.
+  destruct (incl_dec _ l1 l2); easy.
+Qed.
+
+Ltac solve_incl ::= 
+  solve [auto with utils
+        | apply use_compute_incl_compiler; vm_compute; reflexivity
+        | apply use_compute_incl_lang; vm_compute; reflexivity].
+
+
+Lemma full_cps_compiler_preserving
+  : preserving_compiler
+      (heap_cps_ops
+         ++ fix_cps_lang
+         ++ cps_lang
+         ++ cps_prod_lang
+         ++ unit_lang
+         ++ heap
+         ++ nat_exp
+         ++ nat_lang
+         ++ block_subst
+         ++ value_subst)
+      (fix_cps++ cps ++ heap_ctx_cps ++ Ectx_cps++ heap_cps++heap_id++cps_subst++[])
+      (SimpleVFix.fix_lang++SimpleVSTLC.stlc++ heap_ctx++ eval_ctx++heap_ops++(unit_lang ++ heap ++ nat_exp ++ nat_lang)++(exp_subst ++ value_subst)++[]).
+Proof.
+  eapply elab_compiler_implies_preserving.
+  repeat eapply elab_compiler_prefix_implies_elab; eauto with elab_pfs auto_elab.
+  all: solve [use_preserving_hint].
+Qed.  
+
+(*TODO: handle forget discrepancy*)
+Lemma full_cc_compiler_preserving
+  : preserving_compiler
+      (heap_cps_ops ++ heap ++ nat_exp ++ nat_lang
+            ++ cc_lang ++ forget_eq_wkn'
+            ++ unit_eta ++ unit_lang
+            ++ prod_cc ++ cps_prod_lang
+            ++ block_subst ++ value_subst)
+      (heap_cc++heap_id'++cc++prod_cc_compile++ subst_cc++[])
+      (heap_cps_ops++(unit_lang ++ heap ++ nat_exp ++ nat_lang)++cps_lang++cps_prod_lang++(block_subst ++ value_subst)++[]).
+Proof.
+  eapply elab_compiler_implies_preserving.
+  repeat eapply elab_compiler_prefix_implies_elab; eauto with elab_pfs auto_elab.
+  
+  all: try solve [use_preserving_hint].
+  admit.
+Admitted.  
+
+(*TODO: let expressions too*)
+Definition swapfun :=
+  {{e #"lambda" #"nat"
+      (#"let" (#"get" {ovar 0})
+      (#"lambda" #"nat"
+        (#"let" (#"get" {ovar 0})
+          (#"let" (#"set" {ovar 3} {ovar 0})
+            (#"set" {ovar 2} {ovar 3})))))}}.
+
+Definition heap_swap :=
+  {{e #"config" (#"hset" (#"hset" "H" "l" "n'") "l'" "m")
+      (#"app" (#"app" {swapfun} (#"nv" "l")) (#"nv" "l'"))}}.
