src/named/SimpleVCCHeap.v
@@ -1,0 +1,168 @@
+Set Implicit Arguments.
+Set Bullet Behavior "Strict Subproofs".
+
+Require Import String List.
+Import ListNotations.
+Open Scope string.
+Open Scope list.
+From Utils Require Import Utils.
+From Named Require Import Core Compilers Elab ElabCompilers ElabCompilersWithPrefix
+     SimpleVSubst SimpleVCPS SimpleEvalCtx SimpleEvalCtxCPS SimpleUnit NatHeap SimpleVCPSHeap SimpleVCC Matches.
+Import Core.Notations.
+(*TODO: repackage this in compilers*)
+Import CompilerDefs.Notations.
+
+Require Coq.derive.Derive.
+
+(*TODO: make this divide more sensible*)
+Definition heap_id'_def : compiler :=
+  match # from (unit_lang ++ heap ++ nat_exp++ nat_lang) with
+  | {{s #"heap"}} => {{s#"heap"}}
+  end.
+
+
+
+
+Derive heap_id'
+       SuchThat (elab_preserving_compiler subst_cc
+                                          (heap_cps_ops (*TODO: remove via lemma*)
+                                             ++ cc_lang (*TODO: remove via lemma*)
+                                             ++ prod_cc
+                                             ++ cps_prod_lang
+                                             ++ unit_lang
+                                             ++ heap
+                                             ++ nat_exp
+                                             ++ nat_lang
+                                             ++ block_subst
+                                             ++ value_subst)
+                                          heap_id'_def
+                                          heap_id'
+                                          (unit_lang ++ heap ++ nat_exp++ nat_lang))
+       As heap_id'_preserving.
+Proof.
+  auto_elab_compiler.
+  cleanup_elab_after eredex_steps_with heap "heap_comm".
+  cleanup_elab_after eredex_steps_with heap "lookup_miss".
+  cleanup_elab_after eredex_steps_with heap "lookup_empty".
+Qed.
+#[export] Hint Resolve heap_id'_preserving : elab_pfs.
+
+
+(*TODO: move to value_subst? could conflict w/ cmp_forget
+  not currently used
+TODO: variant of one in SimpleVCC.v
+*)
+(*TODO: generalize? reverse for tactics?*)
+Definition forget_eq_wkn'_def : lang :=
+  {[l
+      [:= "G" : #"env", "A" : #"ty"
+         ----------------------------------------------- ("forget_eq_wkn")
+         #"cmp" #"wkn" #"forget" = #"forget"
+         : #"sub" (#"ext" "G" "A") #"emp"
+      ]
+  ]}.
+Derive forget_eq_wkn'
+       SuchThat (Pre.elab_lang value_subst
+                               forget_eq_wkn'_def
+                               forget_eq_wkn')
+       As forget_eq_wkn'_wf.
+Proof. auto_elab. Qed.
+#[export] Hint Resolve forget_eq_wkn'_wf : elab_pfs.
+
+Definition heap_cc_def : compiler :=
+  match # from heap_cps_ops with
+  | {{s #"configuration" "G"}} =>
+    {{s #"configuration" (#"ext" #"emp" "G")}}
+  | {{e #"config" "H" "G" "A" "e"}} =>
+    {{e #"config" "H" "e"}}
+  | {{e #"get" "G" "v" "e"}} =>
+    {{e #"get" "v" (#"blk_subst" (#"snoc" #"forget" (#"pair" {ovar 1} #"hd")) "e")}}
+  | {{e #"set" "G" "v" "v'" "e" }} =>
+    {{e #"set" "v" "v'" "e" }} 
+  end.    
+
+(*TODO: make proof brief*)
+Derive heap_cc
+       SuchThat (elab_preserving_compiler (heap_id'++subst_cc)
+                                          (heap_cps_ops
+                                             ++ cc_lang
+                                             ++ prod_cc
+                                             ++ forget_eq_wkn'
+                                             ++ cps_prod_lang
+                                             ++ unit_lang
+                                             ++ heap
+                                             ++ nat_exp
+                                             ++ nat_lang
+                                             ++ block_subst
+                                             ++ value_subst)
+                                          heap_cc_def
+                                          heap_cc
+                                          heap_cps_ops)
+       As heap_cc_preserving.
+Proof.
+  auto_elab_compiler.
+  {
+    reduce.
+    eapply eq_term_trans.
+    eredex_steps_with heap_cps_ops "eval get".
+    reduce.
+    repeat (term_cong; try term_refl; compute_eq_compilation).
+    eapply eq_term_trans.
+    eapply eq_term_sym.
+    eredex_steps_with forget_eq_wkn' "forget_eq_wkn".
+    compute_eq_compilation.
+    eapply eq_term_trans.
+    2:eredex_steps_with value_subst "id_right".
+    by_reduction.
+  }
+  {
+    reduce.
+    repeat (term_cong; try term_refl; compute_eq_compilation).
+    eapply eq_term_trans; cycle 1.
+    Ltac estep_under lang rule :=
+      eredex_steps_with lang rule
+      || (compute_eq_compilation; term_cong; (estep_under lang rule|| term_refl)).
+
+    Ltac eredex_steps_with lang name ::=
+  let mr := eval vm_compute in (named_list_lookup_err lang name) in
+  lazymatch mr with
+  | Some (term_eq_rule ?c ?e1p ?e2p ?tp) =>
+      lazymatch goal with
+      | |- eq_term ?l ?c' ?t ?e1 ?e2 =>
+            let s := open_constr:((_ : subst)) in
+            (first [ unify_var_names s c | fail 100 "could not unify var names" ]); (first
+             [ replace (eq_term l c' t e1 e2) with (eq_term l c' tp [/s /] e1p [/s /] e2p [/s /]);
+                [  | f_equal; vm_compute; reflexivity ]
+             | fail 2 "could not replace with subst" ]);
+             eapply (eq_term_subst (l:=l) (c:=c') (s1:=s) (s2:=s) (c':=c));
+             [ try (solve [ cleanup_auto_elab ])
+             | eapply eq_subst_refl; try (solve [ cleanup_auto_elab ])
+             | eapply (eq_term_by l c name tp e1p e2p); try (solve [ cleanup_auto_elab ]) ]
+      end
+  | None => fail 100 "rule not found in lang"
+  end; repeat t.
+    Ltac rewrite_leftwards lang name :=
+      first [ eapply eq_term_trans; [estep_under lang name |]
+            | eapply eq_term_trans; [|estep_under lang name ]];
+      compute_eq_compilation.
+    estep_under forget_eq_wkn' "forget_eq_wkn".
+    compute_eq_compilation.
+    eapply eq_term_trans; cycle 1.
+    estep_under value_subst "cmp_snoc".
+    compute_eq_compilation.
+    eapply eq_term_trans; cycle 1.
+    estep_under forget_eq_wkn' "forget_eq_wkn".
+    compute_eq_compilation.
+    eapply eq_term_trans; cycle 1.
+    estep_under value_subst "id_emp_forget".
+    compute_eq_compilation.
+    eapply eq_term_trans; cycle 1.
+    eapply eq_term_sym.
+    estep_under value_subst "id_right".
+    compute_eq_compilation.
+    by_reduction.
+  }
+  Unshelve.
+  all: repeat t'.
+Qed.
+#[export] Hint Resolve heap_cc_preserving : elab_pfs.
